\documentclass{article}

\usepackage{fancyhdr}
\usepackage{extramarks}
\usepackage{amsmath}
\usepackage{amsthm}
\usepackage{amssymb}
\usepackage{amsfonts}

\newcommand{\w}[0]{\omega}
\newcommand{\z}[0]{\zeta}
\newcommand{\Q}[0]{\mathbb{Q}}
\newcommand{\Z}[0]{\mathbb{Z}}
\newcommand{\zquad}[1]{\mathbb{Z}[\sqrt{#1}]}
\newcommand{\qext}[1]{\mathbb{Q}[#1]}
\newcommand{\zext}[1]{\mathbb{Z}[#1]}
\newcommand{\trace}[1]{\text{Tr}(#1)}
\newcommand{\norm}[1]{\text{N}(#1)}
\newcommand{\disc}[1]{\text{disc}(#1)}

\begin{document}

\section*{Chapter 2}

\begin{enumerate}

\item[1]
\begin{enumerate}
    \item[(a)] Show every number field of degree 2 over $\mathbb{Q}$ is one of the quadratic fields.

    Let $K$ be a number field of degree 2, and $f(x) = x^2 + px + q$ be its minimum polynomial over $\mathbb{Q}$.  Since $p, q \in \mathbb{Q}$ we can multiply through to clear the denominators and give us a polynomial $g(x) = ax^2 + bx + c$ over $\mathbb{Z}$ with the same roots as $f(x)$.  Therefore $K = \mathbb{Q}[\sqrt{b^2 - 4ac}]$ is a quadratic field for $m = b^2 - 4ac$.

    \item[(b)] Suppose $K = \mathbb{Q}[\sqrt{m}]$ contains $\sqrt{n}$ for $n$ a squarefree integer.  Since $K$ has the basis $\{1, \sqrt{m}\}$, so $\sqrt{n} = p + q\sqrt{m}$ for $p, q \in \mathbb{Q}$. Therefore $n = p^2 + 2pq\sqrt{m} + q^2m$, so either $p = 0$ or $q = 0$.

    If $p = 0$, then $\sqrt{n} = q\sqrt{m}$ and so $\sqrt{n} / \sqrt{m} = q$.  This can only happen if $q = 1$, meaning $m = n$.

    If $q = 0$, then $\sqrt{n} = p$, which can only happen if $p$ is also an integer, contradicting $n$ squarefree.

    Therefore the quadratic fields are each distinct.
\end{enumerate}

\item[2]
    Let $I$ be the ideal generated by $2$ and $1 + \sqrt{-3}$ in the ring $\mathbb{Z}[\sqrt{-3}]$.

    We have $I \neq (2)$ because $1 + \sqrt{-3}$ ($\in I$) does not have the form $2a + b\sqrt{-3}$ for $a, b \in \mathbb{Z}$.  The ideal $I^2$ is generated by $(4, 2 + 2\sqrt{-3}, -2 + 2\sqrt{-3})$.  The number $-2 + 2\sqrt{-3} = 2 + 2\sqrt{-3} - 4$ and so is redundant as a generator; therefore $I^2 = (4, 2 + 2\sqrt{-3}) = 2I$.

    Since $I^2 = 2I$, prime factorization of ideals in $\mathbb{Z}[\sqrt{-3}]$ must not hold; if we did then $I$ would be invertible, meaning it could be cancelled from the right-hand-side of each equality, giving us $I = (2)$ which is not true (from above).

    Suppose $P$ is a prime ideal of $\mathbb{Z}[\sqrt{-3}]$ containing $2$.  Then $4 \in P$ also.  Since $(1 + \sqrt{-3})(1 - \sqrt{-3}) = 4$ and $P$ is a prime ideal, one of $1 + \sqrt{-3}$ and $1 - \sqrt{-3}$ are also in $P$.  However, if $1 - \sqrt{-3} \in P$ then $1 + \sqrt{-3} \in P$ since $-1 \cdot (1 - \sqrt{-3}) + 2 = 1 + \sqrt{-3}$.  Therefore any prime ideal containing $(2)$ also contains $I$ and $I$ is the unique prime ideal that contains $(2)$.  Since $I$ cannot be expressed as a product of prime ideals, neither can $(2)$.

    (We should expect this; $\mathbb{Z}[\sqrt{-3}]$ is an order of conductor $2$ in $\mathbb{Z}[\frac{1 + \sqrt{-3}}{2}]$ and $I$ is not prime to the conductor, meaning it is not invertible.)

\item[3]
    Complete the proof of Corollary 2, Theorem 1.

    The statement of the text leaves off with $\alpha$ being an algebraic integer if and only if $2r$ and $r^2 - ms^2$ are both integers, where $r, s \in \mathbb{Q}$.

    $2r$ being an integer requires that $r = \frac{a}{2}$, where $a$ is an integer.  Substituting $r = \frac{a}{2}$ into the second equation, we see that $a^2 - 4ms^2$ is an integer divisible by $4$.  In order for the quantity to be an integer, $s = \frac{b}{2}$, where $b$ is an integer.  Therefore $\alpha$ is an algebraic integer of the form $\frac{a + b\sqrt{m}}{2}$ if and only if $a^2 - mb^2 = 0 \mod 4$.

    We finish by considering $m \mod 4$ and seeing under which statements the given equation is solvable.  The key is that integer squares are either equivalent to 0 or 1 modulo 4.
    \begin{itemize}
        \item {\bf $m \equiv 1 \mod 4$}:  Let $a$ be even - then $a^2 \equiv 0 \mod 4$, and to satisfy the equality, $b^2 \equiv 0 \mod 4$ and so $b$ must also be even.  Similarly, if $a$ is odd, then $a^2 \equiv 1 \mod 4$ - to satisfy the equality, $b$ must also be odd.  Therefore $\alpha = \frac{a + b\sqrt{m}}{2}$ for all $a \equiv b\ (2)$ as required.
        \item {\bf $m \equiv 2, 3 \mod 4$}: For the equation to be solvable, both $a$ and $b$ must be equivalent to 0 or 2 modulo 4 (and so even), meaning $\alpha = c + d\sqrt{m}$ for $c, d \in \mathbb{Z}$ as required.
    \end{itemize}

\item[4]
    Suppose $a_0, \ldots, a_{n_1}$ are algebraic integers and $\alpha$ is a complex number satisfiying $\alpha^n + a_{n-1}\alpha^{n-1} + \cdots + a_1\alpha + a_0 = 0$.  Show the ring $\mathbb{Z}{[a_0, \ldots, a_{n-1}, \alpha]}$ has a finitely generated additive group.

    For each $a_i$ let $k_i$ be the degree of the algebraic integer $a_i$ over $\mathbb{Q}$: therefore for any power $k >= k_i$, it can be written as a linear combination of powers of $a_i$ less than $k_i$.  Additionally any power of $\alpha^k$ where $k \ge n$ can be written as a linear combination of powers of $\alpha$ multiplied by each of the $a_i$.  Therefore only a finite number of powers of $a_0^{m_0} \cdots a_n^{m_n} \alpha^{m}$ are needed; the $a_i$ terms are capped to be lower than $k_i$ and the $\alpha$ term is capped to be lower than $n$.

    Since $\alpha$ is a member of a subring of $\mathbb{C}$ that is finitely generated, $\alpha$ is therefore an algebraic integer.

\item[5]
    Let $f$ be a polynomial over $\mathbb{Z}_p$ where $p$ is a prime.  We prove $f(x^p) = (f(x))^p$ by induction on number of terms.

    If $f(x) = kx^{b}$ where $k \in \mathbb{Z}_p$, then $f(x^p) = kx^{pb} = k^p x^{bp} = (kx^{b})^p$ (since $k^p = k$ for all $k \in \mathbb{Z}_p$).

    Next, let $f(x) = g(x) + h(x)$ where $g(x)$ and $h(x)$ have fewer terms than $f(x)$.
    \begin{eqnarray*}
        f(x)^p          &=& (g(x) + h(x))^p \\
                        &=& g(x)^p + h(x)^p + \sum_{k = 1} \binom{p}{k} g(x)^{k} h(x)^{p - k} \\
                        &=& g(x)^p + h(x)^p \\
                        &=& g(x^p) + h(x^p) \text{ (using the inductive hypothesis)}\\
                        &=& f(x^p)
    \end{eqnarray*}
    This is the required result.

\item[6] If $f$ and $g$ are polynomials over a field $K$ and $f^2 \mid g$, then $g = f^2 h$.  Therefore $g' = f^2 h' + 2 h f f'$, so $f \mid g'$.

\item[7] Complete the proof of Corollary 2, Theorem 3.

Let $\phi_{k}$ be the automorphism of $\mathbb{Q}[\omega]$ sending $\omega$ to $\omega^k$.  Then $(\phi_{a} \circ \phi_{b}) (\omega) = (\omega^{a})^{b} = \omega^{ab} = \phi_{ab}$, giving the required result that composition of automorphisms corresponds to multiplication modulo $m$.

\item[8]
\begin{enumerate}
    \item[(a)] Let $\w = e^{2\pi i/p}$ where $p$ is an odd prime.
    Then \[ \text{disc}(\w) = \prod_{1 \le r < s \le n} (\alpha_r - \alpha_s)^2 = \pm p^{p - 2} \]
    Therefore \[ \Big\lvert \prod_{1 \le r < s \le n} (\alpha_r - \alpha_s)\ \Big\rvert = \sqrt{\pm p^{p - 2}} = p^{(p - 3) / 2} \sqrt{\pm p} \]

    Let $\z = e^{2\pi i /3}$.  Using the above we have the identity $(\z - \z^2) = \sqrt{-3}$.

    Let $\z = e^{2\pi i / 5}$.  Note $\z^4 = -(\z^3 + \z^2 + \z + 1)$.

    We expand the product: \[ (\z - \z^2)(\z - \z^3)(\z - z^4)(\z^2 - \z^3)(\z^2 - \z^4)(\z^3 - \z_4) = 10\z^3 + 10\z^2 + 1 \]

    Observing that this product is negative we flip the signs and divide by $5^{(5 - 3)/2} = 5$ to get the identity $\sqrt{5} = -2\z^3 - 2\z^2 - 1$.

    \item[(b)] The 8th cyclotomic polynomial is $x^4 + 1$, so the 8th cyclotomic field contains all the roots of this equation, which includes $\sqrt{i} = (1/\sqrt{2})(1 + i)$ and its complex conjugate $(1/\sqrt{2})(1 - i)$.  Thus the 8th cyclotomic field also contains their sum $2 / \sqrt{2} = \sqrt{2}$.

    \item[(c)] Let $m$ be a squarefree number.  Then $m$ can be written as $2^{i} q$ where $2 \nmid q$, and $i \in \{0, 1\}$.  We proceed by case analysis, showing for each that $\sqrt{m}$ is contained in the $d$th cyclotomic field, where $d = \text{disc}(\mathbb{A} \cap \mathbb{Q}[\sqrt{m}])$.

    $m = -1$: $\sqrt{-1}$ is contained in the 4th cyclotomic field which contains the complex unit $i$ ($d = -4$).

    $m = 2$: $\sqrt{2}$ is contained in the 8th cyclotomic field by part (b) ($d = 4\cdot 2 = 8$).

    $m = -2$: The 8th cyclotomic field contains $i$ (since it contains the 4th cyclotomic field as a subfield) so it contains $\sqrt{-2} = i\sqrt{2}$ ($d = 4\cdot -2 = -8$).

    $m = q$ where $q \equiv 1 \mod 4$: Because $q \equiv 1 \mod 4$, $q$ has an even number of prime factors $\equiv 3 \mod 4$, meaning that $\sqrt{q}$ must be contained in the $q$-th cyclotomic field ($d = q$ since $q\equiv 1\mod 4$).

    $m = q$ where $q \equiv 3 \mod 4$: The $4q$-th cyclotomic field contains the $q$-th cyclotomic field (containing $\sqrt{-q}$) and the 4th cyclotomic field (containing $\sqrt{-1}$) ($d = 4q$ since $q \equiv 3 \mod 4$), and so contains $\sqrt{q}$.

    $m = 2q$ where $q$ is a product of odd primes:  Here $d = 8q$.  By the above, $\sqrt{q}$ is contained in either the $q$-th or $4q$-th cyclotomic field, depending on its residue mod 4.  Thus $\sqrt{2q}$ is contained in the $8q$-th cyclotomic field.

    This shows every quadratic field $\mathbb{Q}[\sqrt{m}]$ is contained within the $d$-th cyclotomic field.
\end{enumerate}

\item[9] Let $\theta$ be a primitive $k$-th root of unity, i.e. $\theta = e^{2\pi i / k}$.  Let $\text{gcd}(k, m) = d$.  Using Euclid's extended algorithm we can find $u, v$ such that $uk + vm = d$.  Then we have
\[ \w^u \theta^v = e^{(2\pi i u)/m} e^{(2\pi i v) / k} = e^{2\pi i (uk + vm) / km} = e^{2\pi i d / km} = e^{2\pi i / r} \]
where $r = \text{lcm}(k, m)$ ($\text{lcm}(k, m) = km / \text{gcd}(k, m)$).

\item[10] Show if $m$ is even, $m \mid r$, and $\phi(r) \le \phi(m)$ then $r = m$.

If $m \mid r$ there is some $k$ such that $mk = r$.  Let $d = \gcd(k, m)$, so $r = mdj$ with $j$ satisfiying $\gcd(j, m) = 1$.  Therefore $\phi(r) = \phi(md)\phi(j)$.  Since $d \mid m$, $\phi(md) = d \cdot \phi(m)$, so \[ \phi(r) = d \cdot \phi(m)\phi(j) \le \phi(m) \]  The inequality forces $d = 1$ and $\phi(j) = 1$.  Because $2 \mid m \mid r$, $\phi(j) = 1$ implies $j = 1$.  Therefore $m = r$.

\item[11]
\begin{enumerate}
    \item[(a)] Suppose all the roots to a monic polynomial $f$ have absolute value $1$.  Show that the coefficient of $x^r$ has absolute value $\le \binom{n}{r}$, where $n$ is the degree of $f$ and $\binom{n}{r}$ is the binomial coefficient.

    Factor $f$ as $f = (x - \alpha_0) \cdots (x - \alpha_n)$.  Re-expanding $f$ we see that the coefficient of $x^r$ is equal to $\sum_{S \subseteq \{0, \ldots, n\}, |S| = r} x^r \prod_{i \in S} \alpha_i$.  By assumption $|\alpha_i| = 1$ for all $i$, so $|\prod_{i \in S} \alpha_i| = 1$.  There are $\binom{n}{r}$ of these subsets of $S$.

    Using the identity $|a + b| \le |a| + |b|$ we have:

    \begin{eqnarray*}
        \left|\sum_{S \subseteq \{0, \ldots, n\}, |S| = r} \prod_{i \in S} \alpha_i \right| &\le& \sum_{S \subseteq \{0, \ldots, n\}, |S| = r} | \prod_{i \in S} \alpha_i | \\
        &\le& \sum_{S \subseteq \{0, \ldots, n\}, |S| = r} 1 \\
        &\le& \binom{n}{r}
    \end{eqnarray*}

    \item[(b)] We will consider all monic polynomials $f$ of degree $n$ and show that only a finite number of them can have a root $\alpha$ all of whose conjugates have absolute value 1.

    By Theorem 1, if $\alpha$ is an algebraic integer, than the coefficients of $f$ are integers.  By (b), the absolute value of the coefficients of $f$ are bounded above $\binom{n}{r}$, therefore there are at most $2\binom{n}{r}$ choices for each coefficient beyond the $x^n$th term.  The constant term of the polynomial must be 1 (since $\alpha$ has absolute value 1) and the first term of the polynomial must also be 1 (since $f$ is monic). This gives an upper bound of $\sum_{r=1}^{n - 1} 2\binom{n}{r} = 2(2^n - 2) = 4(2^{n-1} - 1)$ on the number of algebraic integers satisfying the given condition.

    \item[(c)] TODO
\end{enumerate}

\item[12]
\begin{enumerate}
    \item[(a)] Let $u$ be a unit in $\Z[\w]$, where $\w = e^{2\pi i / p}$.  Show $u / \overline{u}$ is a root of 1.

    The field $\Q[\w]$ has Galois group $\simeq \Z_p^{\times}$, which has cardinality $p - 1$ and so has an element of order 2 (complex conjugation).  Therefore $u$ has $p - 1$ conjugates, which consist of $(p - 1) / 2$ elements along with their complex conjugates.  Enumerate the conjugates of $u$ as $a_1, \ldots, a_n, \overline{a_1}, \ldots, \overline{a_n}$.

    Therefore, the conjugates of $u / \overline{u}$ have the form $a_i / \overline{a_i}$ or $\overline{a_i} / a_i$.  Multiplying over all conjugates of $u / \overline{u}$, we have $\prod_{i = 0}^{n} a_i / \overline{a_i} \cdot \prod_{i = 0}^{n} \overline{a_i} / a_i = 1$, and so $u / \overline{u}$ and all its conjugates have absolute value 1.  By 11 (c), $u / \overline{u}$ is then a root of 1, and so has form $\pm \omega^{k}$.

    \item[(b)] Suppose $u / \overline{u} = -\omega^{k}$.  We derive a contradiction.  Raising both sides to the $p$-th power we have $u^p / \overline{u^p} = -(\omega^{k})^p = -(\omega^{p})^k = -1$, and so $u^p = -\overline{u^p}$.  By exercise 1.25, $u^p \equiv a\ (p)$ for some $a \in \Z$.  Applying exercise 1.23, we see $\overline{u^p} \equiv \overline{a} = a\ (p)$, and so $a \equiv -a\ (p)$.  There $a$ must be 0, and $u^p \equiv 0\ (p)$, so $p$ divides $u^p$.  This contradicts $u^p$ being a unit, since if $p$ divided $u^p$, p would also divide the absolute value of $u^p$, which is 1.  Therefore $u / \overline{u} = \omega^{k}$.
\end{enumerate}

\item[13] Show that 1 and -1 are the only units in the ring $A \cap \Q[\sqrt{m}]$, $m$ squarefree and $m < 0, m \neq -1, -3$.  What if $m = -1, -3$?

Let $u$ be a unit in $A \cap \Q[\sqrt{m}]$.  Then $u = a + b\sqrt{m}$ where $p, q \in A \cap \Q[sqrt{m}]$. Since $N(u) = 1$, then $(a + b\sqrt{m})(a - b\sqrt{m}) = a^2 - b^2 m = 1$.  We proceed by cases on whether $m \equiv 1 \mod 4$.

If $m \not\equiv 1 \mod 4$, then $a$ and $b$ must be integers and so $a^2 - b^2 m = 1$ can only be satisfied if one of the terms is 1 and the other is 0.  If $a^2 = 1$, then $b^2 m = 0$.  This corresponds to the units 1 and -1 in $A \cap \Q[\sqrt{m}]$.  If $-b^2 m = 1$, then $b^2 m = -1$ and so $m = -1$.  This corresponds to the units $i$ and $-i$ in $A \cap \Q[\sqrt{-1}]$.

If $m \equiv 1 \mod 4$ then let $a = r / 2$ and $b = s / 2$.  Therefore $r^2 - s^2 m = 4$.  Since $m$ is negative, both $r^2$ and $-s^2 m$ must be positive.  $r^2$ must be either $0$, $1$, or $4$.

If $r^2$ is 0 then $-s^2 m = 4$, so $s^2 m = -4$, forcing $m = -1$ which is not $\equiv \mod 4$.  (We have considered this case already.)

If $r^2$ is 1 then $-s^2 m = 3$ so $s^2 m = -3$ and $m = -3$, $s = \pm 1$.  This corresponds to the unit $\pm \frac{1}{2} \pm \frac{\sqrt{-3}}{2}$ in the ring $A \cap \Q[\sqrt{-3}]$.

If $r^2$ is 4 then $- s^2 m = 0$, which corresponds to the unit $\pm 1$ in the ring $A \cap \Q[\sqrt{m}]$.

\item[14] Show that $1 + \sqrt{2}$ is a unit in $\mathbb{Z}[\sqrt{2}]$, but not a root of 1.

$1 + \sqrt{2}$ is a unit, as $-(1 - \sqrt{2})$ is its inverse: \[ -(1 + \sqrt{2})(1 - \sqrt{2}) = -1 + (\sqrt{2})^2 = 1 \]

If $1 + \sqrt{2}$ were a root of 1, we would have $(1 + \sqrt{2})^k = 1$ for some $k$.  However by the Binomial Theorem, $(1 + \sqrt{2})^k = \sum^{k}_{i = 0} \binom{k}{i} (\sqrt{2})^i$, which will always contains a term $\sqrt{2}$ multiplied by a positive number.  Therefore $1 + \sqrt{2}$ is not a root of 1.

Let $(1 + \sqrt{2})^k = a + b\sqrt{2}$.  The inverse of this term is \[((1 + \sqrt{2})^k)^{-1} = ((1 + \sqrt{2})^{-1})^{k} = (-1)^k (1 - \sqrt{2})^k = (-1)^k (a - b\sqrt{2})^k \]

Therefore, $(a + b\sqrt{2})^k \cdot (a - b\sqrt{2})^k = \pm 1$ and so the powers of $1 + \sqrt{2}$ give an infinite number of $a$, $b$ such that $a^2 - 2b^2 = \pm 1$.

\item[15]
\begin{itemize}
    \item[(a)] Let $a + b\sqrt{-5}$ be an element of $\zquad{-5}$.  Then the norm of $a + b\sqrt{-5}$ is $(a + b\sqrt{-5})(a - b\sqrt{-5}) = a^2 + 5b^2$, where $a, b \in \mathbb{Z}$.  Since there are no integer solutions $a, b$ such that $a^2 + 5b^2 = 2$ or $a^2 + 5b^2 = 3$, there can be no element of $\zquad{-5}$ with a norm of $2$ or $3$.
    \item[(b)] In $\zquad{-5}$, $6 = 2 \cdot 3 = (1 + \sqrt{-5})(1 - \sqrt{-5})$.  If unique factorization held in $\zquad{-5}$, there would be elements $a, b, c, d \in \zquad{-5}$ such that $a \cdot b = 2$, $c \cdot d = 3$, $a \cdot d  =  1 + \sqrt{-5}$, $b \cdot c = 1 - \sqrt{-5}$.
    However by (a), 2 and 3 are irreducible in $\zquad{-5}$, meaning they are irreducible elements, and so no $a, b, c, d$ can exist.
\end{itemize}

\item[16]
We argue in the style of K. Conrad: Trace and Norm, Section 4.  Suppose $\sqrt{3} \in \qext{\alpha}$ where $\alpha = \sqrt[4]{2}$; therefore $\sqrt{3} = a + b\alpha + c\alpha^2 + d\alpha^3$.  We have the following traces:
\begin{eqnarray*}
    \trace{\sqrt{3}} &=& \sqrt{3} - \sqrt{3} = 0 \\
    \trace{\alpha} &=& \alpha - \alpha + i\alpha - i\alpha = 0\\
    \trace{\alpha^2} &=& \alpha^2 - \alpha^2 + i\alpha^2 - i\alpha^2 = 0\\
    \trace{\alpha^3} &=& \alpha^3 - \alpha^3 + i\alpha^3 - i\alpha^3 = 0\\
\end{eqnarray*}

Since $\sqrt{3} = a + b\alpha + c\alpha^2 + d\alpha^3$,

\begin{eqnarray*}
    \trace{\sqrt{3}} &=& \trace{a + b\alpha + c\alpha^2 + d\alpha^3} \\
    0 &=& a\trace{1} + b\trace{\alpha} + c\trace{\alpha^2} + d\trace{\alpha^3} \\
    0 &=& 4a \\
\end{eqnarray*}

Therefore $a = 0$, and we have $\sqrt{3} = b\alpha + c\alpha^2 + d\alpha^3$.  We have $\trace{\sqrt{3}\alpha} = \trace{\sqrt[4]{9/2}} = \sqrt[4]{9/2} - \sqrt[4]{9/2} + i\sqrt[4]{9/2} - i\sqrt[4]{9/2} = 0$, so $0 = b\trace{1} + c\trace{\alpha} + d\trace{\alpha}^2 = 4b$ and so $b = 0$.

Similarly $\trace{\sqrt{3}/\alpha^2} = \trace{\sqrt{3/2}} = 0$, and so $c = 0$.

From eliminating the coefficients $a, b, c$, we have $d\sqrt[4]{8} = \sqrt{3}$ and so $3 = d^2\sqrt{8} = 2d^2\sqrt{2}$.  Therefore $\sqrt{2}$ is expressible as a rational number $3/d^2$, a contradiction.  Therefore $\sqrt{3} \not\in \qext{\alpha}$.

(Where would this argument break down for $\sqrt{2}$?  $\sqrt{2} = \alpha^2$ so $\sqrt{2} / \alpha^2 = 1$ and so we would conclude that $c = 1$ rather than $c = 0$.)

\item[17] TODO

\item[18] TODO

\item[19] TODO

\item[20] Write $f(x) = (x - \alpha)g(x)$.  By the chain rule $f'(x) = (x - \alpha)g'(x) + g(x)$, so $f'(\alpha) = g(\alpha) = \prod_{\beta \neq \alpha} (\alpha - \beta)$.

\item[21] Let $f(x) = g(x) h(x)$, where $g(x)$ is the minimum polynomial of $\alpha$ over $\mathbb{Z}$.  Then $f'(x) = g'(x)h(x) + g(x) h'(x)$ and $f'(\alpha) = g'(\alpha)h(\alpha)$.  We have \[ \norm{f'(\alpha)} = \norm{g'(\alpha)}\norm{h(\alpha)} \].  By Theorem 8, $\norm{g'(\alpha)} = \pm \disc{\alpha}$, so \[ \norm{f'(\alpha)} = \pm \disc{\alpha}\norm{h(\alpha)} \]
Therefore $\disc{\alpha}$ divides $\norm{f'(\alpha)}$ as required.

\item[33] Let $\w = e^{2\pi i / m}$, where $m \ge 3$.  We know that $N(\w) = \pm 1$ because $\w$ is a unit.  Show the $+$ sign holds.

Write $e^{2\pi i k /m}$ as $\w_k$.  The conjugates of $\w$ have the form $\w_k$ where $(k, m) = 1$.  There are $\phi(m)$ of these, which is even for all $m \ge 3$.  If $\w_k$ is a conjugate, then $\w_{m - k}$ is also a conjugate, since $(k, m) = 1$ implies there exist integers $a, b$ such that $ak + bm = 1$, so $-a(m - k) + (b + a)m = 1$, and so $(m - k, m) = 1$.

For each conjugate $\w_k$, $\w_k \ne \w_{m - k}$; if this were the case, $k = -k \ (m)$, so $2k = 0 \ (m)$ and so $k$ would divide $m$, contradicting $(k, m) = 1$.  Therefore all the conjugates are distinct.

Finally, for each conjugate $\w_{k}$, $\w_k \cdot \w_{m - k} = 1$, so in computing the norm of $\w$, all the conjugates cancel out and the norm of $\w$ is seen to be $1$.


\end{enumerate}

\end{document}

